Add instructions to abstract semanmtics and simulation proof.

src/dafny/AbstractSemantics/AbstractSemantics.dfy
@@ -37,628 +37,481 @@ module AbstractState {
   */
 module AbstractSemantics {
 
-  //   import opened EvmState
-  //   import Bytecode
   import opened AbstractState
 
-  //   function Call(st: EvmState.ExecutingState): (st': EvmState.ExecutingState)
-  //     // ensures st'.CONTINUING? || st' == ERROR(STACK_UNDERFLOW) || st' == ERROR(WRITE_PROTECTION_VIOLATED)
-  //     requires st.Operands() >= 7 // && (st.WritesPermitted() || st.Peek(2) == 0)
-  //     // ensures st' == ERROR(STACK_UNDERFLOW)  <==> st.Operands() < 7
-  //     // ensures st' == ERROR(WRITE_PROTECTION_VIOLATED) <==>
-  //     // st.Operands() >= 7 && !st.WritesPermitted() && st.Peek(2) > 0
-  //     ensures st'.EXECUTING?
-  //     ensures st'.Operands() == st.Operands() - 7 + 1
-  //     ensures st'.Capacity() == st.Capacity() + 7 - 1
-  //     ensures st'.GetStack().contents[1..] == st.GetStack().contents[7..]
-  //     // ensures forall k:: 1 <= k < st'.Operands() ==> st'.Peek(k) == st.Peek(k + 6)
-
-  //     // ensures st'.SlicePeek(1, st'.Operands()) == st.SlicePeek(7, st.Operands())
-  //     ensures st'.PC() == st.PC() + 1
-  //     ensures st'.WritesPermitted() == st.WritesPermitted()
-
-  function Call(s: EState): (s': EState)
-    // requires s.IsValid()
-    // ensures st'.CONTINUING? || st' == ERROR(STACK_UNDERFLOW) || st' == ERROR(WRITE_PROTECTION_VIOLATED)
-    requires s.Operands() >= 7 // && (st.WritesPermitted() || st.Peek(2) == 0)
-    // ensures st' == ERROR(STACK_UNDERFLOW)  <==> st.Operands() < 7
-    // ensures st' == ERROR(WRITE_PROTECTION_VIOLATED) <==>
-    // st.Operands() >= 7 && !st.WritesPermitted() && st.Peek(2) > 0
-    // ensures s'.IsValid()
-    // ensures st'.Operands() == st.Operands() - 7 + 1
-    // ensures st'.Capacity() == st.Capacity() + 7 - 1
-    // ensures st'.GetStack().contents[1..] == st.GetStack().contents[7..]
-    // ensures forall k:: 1 <= k < st'.Operands() ==> st'.Peek(k) == st.Peek(k + 6)
-
-    // ensures st'.SlicePeek(1, st'.Operands()) == st.SlicePeek(7, st.Operands())
-    // ensures st'.PC() == st.PC() + 1
-    // ensures st'.WritesPermitted() == st.WritesPermitted()
+  function Stop(s: EState): (s': EState)
   {
-    EState(s.pc + 1, [0] + s.stack[7..])
+    EState(s.pc + 1, s.stack)
   }
 
-  function StaticCall(s: EState): (s': EState)
-    // requires s.IsValid()
-    // ensures st'.CONTINUING? || st' == ERROR(STACK_UNDERFLOW) || st' == ERROR(WRITE_PROTECTION_VIOLATED)
-    requires s.Operands() >= 6 // && (st.WritesPermitted() || st.Peek(2) == 0)
-    // ensures st' == ERROR(STACK_UNDERFLOW)  <==> st.Operands() < 7
-    // ensures st' == ERROR(WRITE_PROTECTION_VIOLATED) <==>
-    // st.Operands() >= 7 && !st.WritesPermitted() && st.Peek(2) > 0
-    // ensures s'.IsValid()
-    // ensures st'.Operands() == st.Operands() - 7 + 1
-    // ensures st'.Capacity() == st.Capacity() + 7 - 1
-    // ensures st'.GetStack().contents[1..] == st.GetStack().contents[7..]
-    // ensures forall k:: 1 <= k < st'.Operands() ==> st'.Peek(k) == st.Peek(k + 6)
-
-    // ensures st'.SlicePeek(1, st'.Operands()) == st.SlicePeek(7, st.Operands())
-    // ensures st'.PC() == st.PC() + 1
-    // ensures st'.WritesPermitted() == st.WritesPermitted()
-  {
-    EState(s.pc + 1, [0] + s.stack[6..])
-  }
-
-
-  //   lemma SimulationCorrectness(s: EState, n: nat, k: nat, st: ExecutingState)
-  //     ensures Pop.requires(s) &&  s.Abstracts(st) ==> Pop(s).Abstracts(Bytecode.Pop(st))
-  //     ensures Dup.requires(s, k) &&  s.Abstracts(st) ==> Dup(s, k).Abstracts(Bytecode.Dup(st, k))
-  //     ensures Swap.requires(s, k) &&  s.Abstracts(st) ==> Swap(s, k).Abstracts(Bytecode.Swap(st, k))
-  //     ensures MLoad.requires(s) &&  s.Abstracts(st) ==> MLoad(s).Abstracts(Bytecode.MLoad(st))
-  //     ensures MStore.requires(s) &&  s.Abstracts(st) ==> MStore(s).Abstracts(Bytecode.MStore(st))
-  //     ensures Pop.requires(s) &&  s.Abstracts(st) ==> Pop(s).Abstracts(Bytecode.Pop(st))
-  //   {   //  Thanks Dafny
-  //   }
-
-  //   lemma SimulationCorrectnessStackOp(s: EState, n: nat, k: nat, st: ExecutingState)
-  //     requires s.Abstracts(st)
-  //     ensures Bytecode.Pop(st).EXECUTING? ==> Pop.requires(s) && Pop(s).Abstracts(Bytecode.Pop(st))
-  //     ensures k > 0 && Bytecode.Dup(st, k).EXECUTING? ==> Dup.requires(s, k) && Dup(s, k).Abstracts(Bytecode.Dup(st, k))
-  //     ensures 1 <= k <= 16 && Bytecode.Swap(st, k).EXECUTING? ==> Swap.requires(s, k) && Swap(s, k).Abstracts(Bytecode.Swap(st, k))
-  //   {   //  Thanks Dafny
-  //   }
-
-  //   lemma SimulationCorrectnessV2MemOp(s: EState, n: nat, k: nat, st: ExecutingState)
-  //     requires s.Abstracts(st)
-  //     ensures Bytecode.MLoad(st).EXECUTING? ==> MLoad.requires(s) && MLoad(s).Abstracts(Bytecode.MLoad(st))
-  //     ensures Bytecode.MStore(st).EXECUTING? ==> MStore(s).Abstracts(Bytecode.MStore(st))
-  //   {   //  Thanks Dafny
-  //   }
-
-  function PushN(s: EState, n: nat, k: nat): (s': EState)
-    // requires s.IsValid()
-    requires 1 <= n <= 32
-    requires k <= Int.MAX_U256
-    // requires s.Capacity() >= 1
-
-    ensures s'.Operands() == s.Operands() + 1
-    // ensures s'.Capacity() == s.Capacity() - 1
-    ensures s'.stack[1..] == s.stack
-    // ensures s'.IsValid()
-  {
-    EState(s.pc + n + 1, [k as Int.u256] + s.stack)
-  }
-
-  function Push0(s: EState): (s': EState)
-    // requires s.IsValid()
-    // requires s.Capacity() >= 1
-
-    // ensures s'.IsValid()
-    ensures s'.Operands() == s.Operands() + 1
-    // ensures s'.Capacity() == s.Capacity() - 1
-    ensures s'.stack[1..] == s.stack
-  {
-    EState(s.pc + 1, [0] + s.stack)
-  }
-
-  function Pop(s: EState): (s': EState)
-    // requires s.IsValid()
-    requires s.Operands() >= 1
-
-    // ensures s'.IsValid()
-    // ensures s'.Operands() == s.Operands() - 1
-    // ensures s'.Capacity() == s.Capacity() + 1
-  {
-    EState(s.pc + 1, s.stack[1..])
-  }
-
-  function Dup(s: EState, k: nat): (s': EState)
-    // requires s.IsValid()
-    requires s.Operands() >= k > 0
-    // requires s.Capacity() >= 1
-
-    // ensures s'.IsValid()
-    ensures s'.stack == [s.stack[k - 1]] + s.stack
-    // ensures s'.Operands() == s.Operands() + 1
-    // ensures s'.Capacity() == s.Capacity() - 1
-  {
-    EState(s.pc + 1, [s.stack[k - 1]] + s.stack)
-  }
-
-  function Swap(s: EState, k: nat): (s': EState)
-    // requires s.IsValid()
-    requires 1 <= k <= 16
-    requires s.Operands() > k
-
-    // ensures s'.IsValid()
-    // ensures s'.Operands() == s.Operands()
-    // ensures s'.Capacity() == s.Capacity()
-  {
-    EState(s.pc + 1, s.stack[0 := s.stack[k]][k := s.stack[0]])
-  }
-
-  function SLoad(s: EState): (s': EState)
-    // requires s.IsValid()
-    requires s.Operands() >= 1
-
-    // ensures s'.IsValid()
-    ensures s'.Operands() == s.Operands()
-    // ensures s'.Capacity() == s.Capacity()
-  {
-    EState(s.pc + 1, [0] + s.stack[1..])
-  }
-
-  function SStore(s: EState): (s': EState)
-    // requires s.IsValid()
-    requires s.Operands() >= 2
-
-    // ensures s'.IsValid()
-    ensures s'.Operands() == s.Operands() - 2
-    // ensures s'.Capacity() == s.Capacity()
-  {
-    EState(s.pc + 1, s.stack[2..])
-  }
-
-  function MLoad(s: EState): (s': EState)
-    // requires s.IsValid()
-    requires s.Operands() >= 1
-
-    // ensures s'.IsValid()
-    // ensures s'.Operands() == s.Operands()
-    // ensures s'.Capacity() == s.Capacity()
-  {
-    EState(s.pc + 1, [0] + s.stack[1..])
-  }
-
-  function MStore(s: EState): (s': EState)
-    // requires s.IsValid()
-    requires s.Operands() >= 2
-
-    // ensures s'.IsValid()
-    // ensures s'.Operands() == s.Operands() - 2
-    // ensures s'.Capacity() == s.Capacity() + 2
-  {
-    EState(s.pc + 1, s.stack[2..])
-  }
-
-  function MStore8(s: EState): (s': EState)
-    // requires s.IsValid()
-    requires s.Operands() >= 2
-
-    // ensures s'.IsValid()
-    // ensures s'.Operands() == s.Operands() - 2
-    // ensures s'.Capacity() == s.Capacity() + 2
-  {
-    EState(s.pc + 1, s.stack[2..])
-  }
-
-  function Jump(s: EState): (s': EState)
-    // requires s.IsValid()
-    requires s.Operands() >= 1
-    // requires s.stack[0].Value?
-    // ensures s'.IsValid()
-    // ensures s'.Operands() == s.Operands() - 1
-    // ensures s'.Capacity() == s.Capacity() + 1
-  {
-    EState(s.stack[0] as nat, s.stack[1..])
-  }
-
-  function JumpI(s: EState): (s': EState)
-    // requires s.IsValid()
-    requires s.Operands() >= 2
-    // requires s.stack[0].Value?
-    // ensures s'.IsValid()
-    // ensures s'.Operands() == s.Operands() - 1
-    // ensures s'.Capacity() == s.Capacity() + 1
-    ensures s'.pc == s.stack[0] as nat || s'.pc == s.pc + 1
-    ensures s'.stack == s.stack[2..]
-  {
-
-    EState(if s.stack[1] > 0 then s.stack[0] as nat else s.pc + 1 as nat, s.stack[2..])
-  }
+  // Arithmetic op
 
   function Add(s: EState): (s': EState)
-    // requires s.IsValid()
     requires s.Operands() >= 2
-    // ensures s'.IsValid()
-    // ensures s'.Operands() == s.Operands() - 1
-    // ensures s'.Capacity() == s.Capacity() + 1
   {
     EState(s.pc + 1, [0] + s.stack[2..])
   }
 
   function Sub(s: EState): (s': EState)
-    // requires s.IsValid()
     requires s.Operands() >= 2
-    // ensures s'.IsValid()
-    // ensures s'.Operands() == s.Operands() - 1
-    // ensures s'.Capacity() == s.Capacity() + 1
   {
     EState(s.pc + 1, [0] + s.stack[2..])
   }
 
   function Mul(s: EState): (s': EState)
-    // requires s.IsValid()
     requires s.Operands() >= 2
-    // ensures s'.IsValid()
-    // ensures s'.Operands() == s.Operands() - 1
-    // ensures s'.Capacity() == s.Capacity() + 1
   {
     EState(s.pc + 1, [0] + s.stack[2..])
   }
 
   function Div(s: EState): (s': EState)
-    // requires s.IsValid()
     requires s.Operands() >= 2
-    // ensures s'.IsValid()
-    // ensures s'.Operands() == s.Operands() - 1
-    // ensures s'.Capacity() == s.Capacity() + 1
+  {
+    EState(s.pc + 1, [0] + s.stack[2..])
+  }
+
+  function SDiv(s: EState): (s': EState)
+    requires s.Operands() >= 2
   {
     EState(s.pc + 1, [0] + s.stack[2..])
   }
 
   function Mod(s: EState): (s': EState)
-    // requires s.IsValid()
     requires s.Operands() >= 2
-    // ensures s'.IsValid()
-    // ensures s'.Operands() == s.Operands() - 1
-    // ensures s'.Capacity() == s.Capacity() + 1
   {
     EState(s.pc + 1, [0] + s.stack[2..])
+  }
+
+  function SMod(s: EState): (s': EState)
+    requires s.Operands() >= 2
+  {
+    EState(s.pc + 1, [0] + s.stack[2..])
+  }
+
+  function AddMod(s: EState): (s': EState)
+    requires s.Operands() >= 3
+  {
+    EState(s.pc + 1, [0] + s.stack[3..])
+  }
+
+  function MulMod(s: EState): (s': EState)
+    requires s.Operands() >= 3
+  {
+    EState(s.pc + 1, [0] + s.stack[3..])
   }
 
   function Exp(s: EState): (s': EState)
-    // requires s.IsValid()
     requires s.Operands() >= 2
-    // ensures s'.IsValid()
-    // ensures s'.Operands() == s.Operands() - 1
-    // ensures s'.Capacity() == s.Capacity() + 1
   {
     EState(s.pc + 1, [0] + s.stack[2..])
   }
 
-  function Byte(s: EState): (s': EState)
-    // requires s.IsValid()
+  function SignExtend(s: EState): (s': EState)
     requires s.Operands() >= 2
-    // ensures s'.IsValid()
-    ensures s'.Operands() == s.Operands() - 1
-    // ensures s'.Capacity() == s.Capacity() + 1
   {
     EState(s.pc + 1, [0] + s.stack[2..])
   }
+
+  //  Comparison operators
 
   function Lt(s: EState): (s': EState)
-    // requires s.IsValid()
     requires s.Operands() >= 2
-    // ensures s'.IsValid()
-    // ensures s'.Operands() == s.Operands() - 1
-    // ensures s'.Capacity() == s.Capacity() + 1
   {
     EState(s.pc + 1, [0] + s.stack[2..])
   }
 
   function Gt(s: EState): (s': EState)
-    // requires s.IsValid()
     requires s.Operands() >= 2
-    // ensures s'.IsValid()
-    // ensures s'.Operands() == s.Operands() - 1
-    // ensures s'.Capacity() == s.Capacity() + 1
   {
     EState(s.pc + 1, [0] + s.stack[2..])
   }
 
-  function Slt(s: EState): (s': EState)
-    // requires s.IsValid()
+  function SLt(s: EState): (s': EState)
     requires s.Operands() >= 2
-    // ensures s'.IsValid()
-    // ensures s'.Operands() == s.Operands() - 1
-    // ensures s'.Capacity() == s.Capacity() + 1
   {
     EState(s.pc + 1, [0] + s.stack[2..])
   }
 
-   function Sgt(s: EState): (s': EState)
-    // requires s.IsValid()
+  function SGt(s: EState): (s': EState)
     requires s.Operands() >= 2
-    // ensures s'.IsValid()
-    // ensures s'.Operands() == s.Operands() - 1
-    // ensures s'.Capacity() == s.Capacity() + 1
   {
     EState(s.pc + 1, [0] + s.stack[2..])
   }
 
   function Eq(s: EState): (s': EState)
-    // requires s.IsValid()
     requires s.Operands() >= 2
-    // ensures s'.IsValid()
-    // ensures s'.Operands() == s.Operands() - 1
-    // ensures s'.Capacity() == s.Capacity() + 1
   {
     EState(s.pc + 1, [0] + s.stack[2..])
   }
-
-  function Shr(s: EState): (s': EState)
-    // requires s.IsValid()
-    requires s.Operands() >= 2
-    // ensures s'.IsValid()
-    // ensures s'.Operands() == s.Operands() - 1
-    // ensures s'.Capacity() == s.Capacity() + 1
-  {
-    EState(s.pc + 1, [0] + s.stack[2..])
-  }
-
-  function Shl(s: EState): (s': EState)
-    // requires s.IsValid()
-    requires s.Operands() >= 2
-    // ensures s'.IsValid()
-    // ensures s'.Operands() == s.Operands() - 1
-    // ensures s'.Capacity() == s.Capacity() + 1
-  {
-    EState(s.pc + 1, [0] + s.stack[2..])
-  }
-
 
   function IsZero(s: EState): (s': EState)
-    // requires s.IsValid()
     requires s.Operands() >= 1
-    // ensures s'.IsValid()
-    // ensures s'.Operands() == s.Operands() - 1
-    // ensures s'.Capacity() == s.Capacity() + 1
   {
     EState(s.pc + 1, [0] + s.stack[1..])
   }
 
+  // Bitwise op
+
   function And(s: EState): (s': EState)
-    // requires s.IsValid()
     requires s.Operands() >= 2
-    // ensures s'.IsValid()
-    // ensures s'.Operands() == s.Operands() - 1
-    // ensures s'.Capacity() == s.Capacity() + 1
   {
     EState(s.pc + 1, [0] + s.stack[2..])
   }
 
   function Or(s: EState): (s': EState)
-    // requires s.IsValid()
     requires s.Operands() >= 2
-    // ensures s'.IsValid()
-    // ensures s'.Operands() == s.Operands() - 1
-    // ensures s'.Capacity() == s.Capacity() + 1
   {
     EState(s.pc + 1, [0] + s.stack[2..])
   }
-
 
   function Xor(s: EState): (s': EState)
-    // requires s.IsValid()
     requires s.Operands() >= 2
-    // ensures s'.IsValid()
-    // ensures s'.Operands() == s.Operands() - 1
-    // ensures s'.Capacity() == s.Capacity() + 1
   {
     EState(s.pc + 1, [0] + s.stack[2..])
   }
-
 
   function Not(s: EState): (s': EState)
-    // requires s.IsValid()
     requires s.Operands() >= 1
-    // ensures s'.IsValid()
     ensures s'.Operands() == s.Operands()
-    // ensures s'.Capacity() == s.Capacity() + 1
   {
     EState(s.pc + 1, [0] + s.stack[1..])
   }
 
-  function Address(s: EState): (s': EState)
-    // requires s.IsValid()
-    // requires s.Operands() >= 2
-    // requires s.Capacity() >= 1
-    // ensures s'.IsValid()
-    // ensures s'.Operands() == s.Operands() + 1
-    // ensures s'.Capacity() == s.Capacity() - 1
-  {
-    EState(s.pc + 1, [0] + s.stack)
-  }
-
-   function Balance(s: EState): (s': EState)
-    // requires s.IsValid()
-    requires s.Operands() >= 1
-    // requires s.Capacity() >= 1
-    // ensures s'.IsValid()
-    ensures s'.Operands() == s.Operands() 
-    // ensures s'.Capacity() == s.Capacity() - 1
-  {
-    EState(s.pc + 1, [0] + s.stack[1..])
-  }
-
-   function SelfBalance(s: EState): (s': EState)
-    // requires s.IsValid()
-    // requires s.Operands() >= 1
-    // requires s.Capacity() >= 1
-    // ensures s'.IsValid()
-    ensures s'.Operands() == s.Operands() + 1
-    // ensures s'.Capacity() == s.Capacity() - 1
-  {
-    EState(s.pc + 1, [0] + s.stack)
-  }
-
-  function Gas(s: EState): (s': EState)
-    // requires s.IsValid()
-    // requires s.Operands() >= 2
-    // requires s.Capacity() >= 1
-    // ensures s'.IsValid()
-    // ensures s'.Operands() == s.Operands() + 1
-    // ensures s'.Capacity() == s.Capacity() - 1
-  {
-    EState(s.pc + 1, [0] + s.stack)
-  }
-
-  function Keccak256(s: EState): (s': EState)
-    // requires s.IsValid()
+  function Byte(s: EState): (s': EState)
     requires s.Operands() >= 2
-    // requires s.Capacity() >= 1
-    // ensures s'.IsValid()
     ensures s'.Operands() == s.Operands() - 1
-    // ensures s'.Capacity() == s.Capacity() - 1
   {
     EState(s.pc + 1, [0] + s.stack[2..])
+  }
+
+  function Shr(s: EState): (s': EState)
+    requires s.Operands() >= 2
+  {
+    EState(s.pc + 1, [0] + s.stack[2..])
+  }
+
+  function Shl(s: EState): (s': EState)
+    requires s.Operands() >= 2
+  {
+    EState(s.pc + 1, [0] + s.stack[2..])
+  }
+
+  function Sar(s: EState): (s': EState)
+    requires s.Operands() >= 2
+  {
+    EState(s.pc + 1, [0] + s.stack[2..])
+  }
+
+  //  Keccak256
+
+  function Keccak256(s: EState): (s': EState)
+    requires s.Operands() >= 2
+    ensures s'.Operands() == s.Operands() - 1
+  {
+    EState(s.pc + 1, [0] + s.stack[2..])
+  }
+
+  //  Env op
+
+  function Address(s: EState): (s': EState)
+  {
+    EState(s.pc + 1, [0] + s.stack)
+  }
+
+  function Balance(s: EState): (s': EState)
+    requires s.Operands() >= 1
+  {
+    EState(s.pc + 1, [0] + s.stack[1..])
+  }
+
+  function Origin(s: EState): (s': EState)
+  {
+    EState(s.pc + 1, [0] + s.stack)
+  }
+
+  function Caller(s: EState): (s': EState)
+  {
+    EState(s.pc + 1, [0] + s.stack)
   }
 
   function CallValue(s: EState): (s': EState)
-    // requires s.IsValid()
-    // requires s.Capacity() >= 1
-    // ensures s'.IsValid()
-    // ensures s'.Operands() == s.Operands()
-    // ensures s'.Capacity() == s.Capacity()
   {
     EState(s.pc + 1, [0] + s.stack)
   }
 
   function CallDataLoad(s: EState): (s': EState)
-    // requires s.IsValid()
     requires s.Operands() >= 1
-    // ensures s'.IsValid()
-    // ensures s'.Operands() == s.Operands()
-    // ensures s'.Capacity() == s.Capacity()
   {
     EState(s.pc + 1, [0] + s.stack[1..])
   }
 
+  function CallDataSize(s: EState): (s': EState)
+  {
+    EState(s.pc + 1, [0] + s.stack)
+  }
+
   function CallDataCopy(s: EState): (s': EState)
-    // requires s.IsValid()
     requires s.Operands() >= 3
-    // ensures s'.IsValid()
-    // ensures s'.Operands() == s.Operands() - 3
-    // ensures s'.Capacity() == s.Capacity() + 3
   {
     EState(s.pc + 1, s.stack[3..])
+  }
+
+  function CodeSize(s: EState): (s': EState)
+  {
+    EState(s.pc + 1, [0] + s.stack)
   }
 
   function CodeCopy(s: EState): (s': EState)
-    // requires s.IsValid()
     requires s.Operands() >= 3
-    // ensures s'.IsValid()
-    ensures s'.Operands() == s.Operands() - 3
-    // ensures s'.Capacity() == s.Capacity() + 3
   {
     EState(s.pc + 1, s.stack[3..])
   }
 
-  function CallDataSize(s: EState): (s': EState)
-    // requires s.IsValid()
-    // requires s.Capacity() >= 1
-    // ensures s'.IsValid()
-    // ensures s'.Operands() == s.Operands() - 3
-    // ensures s'.Capacity() == s.Capacity() + 3
+  function GasPrice(s: EState): (s': EState)
   {
     EState(s.pc + 1, [0] + s.stack)
   }
 
   function ExtCodeSize(s: EState): (s': EState)
-    // requires s.IsValid()
     requires s.Operands() >= 1
-    // ensures s'.IsValid()
-    ensures s'.Operands() == s.Operands()
-    // ensures s'.Capacity() == s.Capacity() + 3
   {
     EState(s.pc + 1, [0] + s.stack[1..])
   }
-  function Caller(s: EState): (s': EState)
-    // requires s.IsValid()
-    // requires s.Capacity() >= 1
-    // ensures s'.IsValid()
-    // ensures s'.Operands() == s.Operands() + 1
-    // ensures s'.Capacity() == s.Capacity() - 1
-    ensures s'.stack == [0] + s.stack
+
+  function ExtCodeCopy(s: EState): (s': EState)
+    requires s.Operands() >= 4
   {
-    EState(s.pc + 1, [0] + s.stack)
+    EState(s.pc + 1, s.stack[4..])
   }
 
   function ReturnDataSize(s: EState): (s': EState)
-    // requires s.IsValid()
-    // requires s.Capacity() >= 1
-    // ensures s'.IsValid()
-    ensures s'.Operands() == s.Operands() + 1
-    // ensures s'.Capacity() == s.Capacity() + 3
   {
     EState(s.pc + 1, [0] + s.stack)
   }
 
   function ReturnDataCopy(s: EState): (s': EState)
-    // requires s.IsValid()
     requires s.Operands() >= 3
-    // ensures s'.IsValid()
-    ensures s'.Operands() == s.Operands() - 3
-    // ensures s'.Capacity() == s.Capacity() + 3
   {
     EState(s.pc + 1, s.stack[3..])
   }
 
+  function ExtCodeHash(s: EState): (s': EState)
+    requires s.Operands() >= 1
+  {
+    EState(s.pc + 1, [0] + s.stack[1..])
+  }
+
+  //  Block information
+
+  function BlockHash(s: EState): (s': EState)
+    requires s.Operands() >= 1
+  {
+    EState(s.pc + 1, [0] + s.stack[1..])
+  }
+
+  function CoinBase(s: EState): (s': EState)
+  {
+    EState(s.pc + 1, [0] + s.stack)
+  }
+
+  function TimeStamp(s: EState): (s': EState)
+  {
+    EState(s.pc + 1, [0] + s.stack)
+  }
+
+  function Number(s: EState): (s': EState)
+  {
+    EState(s.pc + 1, [0] + s.stack)
+  }
+
+  function Difficulty(s: EState): (s': EState)
+  {
+    EState(s.pc + 1, [0] + s.stack)
+  }
+
+  function GasLimit(s: EState): (s': EState)
+  {
+    EState(s.pc + 1, [0] + s.stack)
+  }
+
+  function ChainID(s: EState): (s': EState)
+  {
+    EState(s.pc + 1, [0] + s.stack)
+  }
+
+  function SelfBalance(s: EState): (s': EState)
+    ensures s'.Operands() == s.Operands() + 1
+  {
+    EState(s.pc + 1, [0] + s.stack)
+  }
+
+  function BaseFee(s: EState): (s': EState)
+    ensures s'.Operands() == s.Operands() + 1
+  {
+    EState(s.pc + 1, [0] + s.stack)
+  }
+
+  //  Stack, memory and storage op
+
+  function Pop(s: EState): (s': EState)
+    requires s.Operands() >= 1
+  {
+    EState(s.pc + 1, s.stack[1..])
+  }
+
+  function MLoad(s: EState): (s': EState)
+    requires s.Operands() >= 1
+  {
+    EState(s.pc + 1, [0] + s.stack[1..])
+  }
+
+  function MStore(s: EState): (s': EState)
+    requires s.Operands() >= 2
+  {
+    EState(s.pc + 1, s.stack[2..])
+  }
+
+  function MStore8(s: EState): (s': EState)
+    requires s.Operands() >= 2
+  {
+    EState(s.pc + 1, s.stack[2..])
+  }
+
+  function SLoad(s: EState): (s': EState)
+    requires s.Operands() >= 1
+    ensures s'.Operands() == s.Operands()
+  {
+    EState(s.pc + 1, [0] + s.stack[1..])
+  }
+
+  function SStore(s: EState): (s': EState)
+    requires s.Operands() >= 2
+    ensures s'.Operands() == s.Operands() - 2
+  {
+    EState(s.pc + 1, s.stack[2..])
+  }
+
+  function Jump(s: EState): (s': EState)
+    requires s.Operands() >= 1
+    // requires s.stack[0].Value?
+  {
+    EState(s.stack[0] as nat, s.stack[1..])
+  }
+
+  function JumpI(s: EState): (s': EState)
+    requires s.Operands() >= 2
+    ensures s'.pc == s.stack[0] as nat || s'.pc == s.pc + 1
+    ensures s'.stack == s.stack[2..]
+  {
+    EState(if s.stack[1] > 0 then s.stack[0] as nat else s.pc + 1 as nat, s.stack[2..])
+  }
+
+  function MSize(s: EState): (s': EState)
+  {
+    EState(s.pc + 1, [0] + s.stack)
+  }
+
+  function Gas(s: EState): (s': EState)
+  {
+    EState(s.pc + 1, [0] + s.stack)
+  }
+
   function JumpDest(s: EState): (s': EState)
-    // requires s.IsValid()
-    // requires s.Capacity() >= 1
-    // ensures s'.IsValid()
-    // ensures s'.Operands() == s.Operands() + 1
-    // ensures s'.Capacity() == s.Capacity() - 1
-    // ensures s'.stack == [0] + s.stack
   {
     EState(s.pc + 1, s.stack)
   }
 
-  function Revert(s: EState): (s': EState)
-    // requires s.IsValid()
-    // requires s.Capacity() >= 1
-    // ensures s'.IsValid()
-    // ensures s'.Operands() == s.Operands() + 1
-    // ensures s'.Capacity() == s.Capacity() - 1
-    // ensures s'.stack == [0] + s.stack
+  function Push0(s: EState): (s': EState)
+    ensures s'.Operands() == s.Operands() + 1
+    ensures s'.stack[1..] == s.stack
   {
-    EState(s.pc + 1, s.stack)
+    EState(s.pc + 1, [0] + s.stack)
   }
 
-  function Return(s: EState): (s': EState)
-    // requires s.IsValid()
-    // requires s.Capacity() >= 1
-    // ensures s'.IsValid()
-    // ensures s'.Operands() == s.Operands() + 1
-    // ensures s'.Capacity() == s.Capacity() - 1
-    // ensures s'.stack == [0] + s.stack
+  function PushN(s: EState, n: nat, k: nat): (s': EState)
+    requires 1 <= n <= 32
+    requires k <= Int.MAX_U256
+    ensures s'.Operands() == s.Operands() + 1
+    ensures s'.stack[1..] == s.stack
   {
-    EState(s.pc + 1, s.stack)
+    EState(s.pc + n + 1, [k as Int.u256] + s.stack)
   }
 
-  function Stop(s: EState): (s': EState)
-    // requires s.IsValid()
-    // requires s.Capacity() >= 1
-    // ensures s'.IsValid()
-    // ensures s'.Operands() == s.Operands() + 1
-    // ensures s'.Capacity() == s.Capacity() - 1
-    // ensures s'.stack == [0] + s.stack
+  function Dup(s: EState, k: nat): (s': EState)
+    requires s.Operands() >= k > 0
+    ensures s'.stack == [s.stack[k - 1]] + s.stack
   {
-    EState(s.pc + 1, s.stack)
+    EState(s.pc + 1, [s.stack[k - 1]] + s.stack)
   }
 
+  function Swap(s: EState, k: nat): (s': EState)
+    requires 1 <= k <= 16
+    requires s.Operands() > k
+  {
+    EState(s.pc + 1, s.stack[0 := s.stack[k]][k := s.stack[0]])
+  }
 
+  //  Log op
   function LogN(s: EState, n: nat): (s': EState)
     requires n <= 4
-    // requires s.IsValid()
     requires s.Operands() >= n + 2
-    // ensures s'.IsValid()
     ensures s'.Operands() == s.Operands() - (n + 2)
-    // ensures s'.Capacity() == s.Capacity() - 1
-    // ensures s'.stack == [0] + s.stack
   {
     EState(s.pc + 1, s.stack[n + 2..])
   }
 
+  //  System op
+
+  function Create(s: EState): (s': EState)
+    requires s.Operands() >= 3
+  {
+    EState(s.pc + 1, [0] + s.stack[3..])
+  }
+
+  function Call(s: EState): (s': EState)
+    requires s.Operands() >= 7
+  {
+    EState(s.pc + 1, [0] + s.stack[7..])
+  }
+
+  function CallCode(s: EState): (s': EState)
+    requires s.Operands() >= 7
+  {
+    EState(s.pc + 1, [0] + s.stack[7..])
+  }
+
+  function Return(s: EState): (s': EState)
+  {
+    EState(s.pc + 1, s.stack)
+  }
+
+  function DelegateCall(s: EState): (s': EState)
+    requires s.Operands() >= 6
+  {
+    EState(s.pc + 1, [0] + s.stack[6..])
+  }
+
+  function Create2(s: EState): (s': EState)
+    requires s.Operands() >= 4
+  {
+    EState(s.pc + 1, [0] + s.stack[4..])
+  }
+
+  function StaticCall(s: EState): (s': EState)
+    requires s.Operands() >= 6
+  {
+    EState(s.pc + 1, [0] + s.stack[6..])
+  }
+
+  function Revert(s: EState): (s': EState)
+  {
+    EState(s.pc + 1, s.stack)
+  }
+
+  function SelfDestruct(s: EState): (s': EState)
+    requires s.Operands() >= 1
+  {
+    EState(s.pc + 1, s.stack[1..])
+  }
 
 }
