src/dafny/AbstractSemantics/AbstractSemanticsWithDafnyEVMInt.dfy
@@ -16,27 +16,27 @@ include "../../../../evm-dafny/src/dafny/state.dfy"
 include "../../../../evm-dafny/src/dafny/util/int.dfy"
 
 /**
- *  This project and the Dafny-EVM both use an Int module.
- *  There is a name clash when we want to mix them together.
- *  For the time being the module in these files are copies
- *  of the absttact semantics but using the Dafny-EVM int instead of
- *  of this project's Int module. 
- *  The two moduels are the same so it is not an issue.
- */
+  *  This project and the Dafny-EVM both use an Int module.
+  *  There is a name clash when we want to mix them together.
+  *  For the time being the module in these files are copies
+  *  of the absttact semantics but using the Dafny-EVM int instead of
+  *  of this project's Int module. 
+  *  The two moduels are the same so it is not an issue.
+  */
 module AbstractStateDafnyEVM {
 
   import opened Int
   import opened EvmState
 
 
-  datatype StackElem = Value(v: Int.u256) | Random() 
+  datatype StackElem = Value(v: Int.u256) | Random()
 
   datatype EState = EState(pc: nat, stack: seq<StackElem>)
   {
     function Operands(): nat { |stack| }
 
     predicate Abstracts(st: ExecutingState) {
-      && st.PC() == pc 
+      && st.PC() == pc
       && st.Operands() == Operands()
       && forall k:: 0 <= k < Operands() && stack[k].Value? ==> stack[k].v == st.GetStack().contents[k]
     }
@@ -50,554 +50,480 @@ module AbstractSemanticsDafnyEVM {
 
   import opened AbstractStateDafnyEVM
 
-  function Call(s: EState): (s': EState)
-    requires s.Operands() >= 7 // && (st.WritesPermitted() || st.Peek(2) == 0)
+  function Stop(s: EState): (s': EState)
   {
-    EState(s.pc + 1, [Random()] + s.stack[7..])
+    EState(s.pc + 1, s.stack)
   }
 
-  function StaticCall(s: EState): (s': EState)
-    requires s.Operands() >= 6 
-  {
-    EState(s.pc + 1, [Random()] + s.stack[6..])
-  }
-
-  function PushN(s: EState, n: nat, k: nat): (s': EState)
-    // requires s.IsValid()
-    requires 1 <= n <= 32
-    requires k <= Int.MAX_U256
-    // requires s.Capacity() >= 1
-
-    ensures s'.Operands() == s.Operands() + 1
-    // ensures s'.Capacity() == s.Capacity() - 1
-    ensures s'.stack[1..] == s.stack
-    // ensures s'.IsValid()
-  {
-    EState(s.pc + n + 1, [Value(k as Int.u256)] + s.stack)
-  }
-
-  function Push0(s: EState): (s': EState)
-    // requires s.IsValid()
-    // requires s.Capacity() >= 1
-
-    // ensures s'.IsValid()
-    ensures s'.Operands() == s.Operands() + 1
-    // ensures s'.Capacity() == s.Capacity() - 1
-    ensures s'.stack[1..] == s.stack
-  {
-    EState(s.pc + 1, [Random()] + s.stack)
-  }
-
-  function Pop(s: EState): (s': EState)
-    // requires s.IsValid()
-    requires s.Operands() >= 1
-
-    // ensures s'.IsValid()
-    // ensures s'.Operands() == s.Operands() - 1
-    // ensures s'.Capacity() == s.Capacity() + 1
-  {
-    EState(s.pc + 1, s.stack[1..])
-  }
-
-  function Dup(s: EState, k: nat): (s': EState)
-    // requires s.IsValid()
-    requires s.Operands() >= k > 0
-    // requires s.Capacity() >= 1
-
-    // ensures s'.IsValid()
-    ensures s'.stack == [s.stack[k - 1]] + s.stack
-    // ensures s'.Operands() == s.Operands() + 1
-    // ensures s'.Capacity() == s.Capacity() - 1
-  {
-    EState(s.pc + 1, [s.stack[k - 1]] + s.stack)
-  }
-
-  function Swap(s: EState, k: nat): (s': EState)
-    // requires s.IsValid()
-    requires 1 <= k <= 16
-    requires s.Operands() > k
-
-    // ensures s'.IsValid()
-    // ensures s'.Operands() == s.Operands()
-    // ensures s'.Capacity() == s.Capacity()
-  {
-    EState(s.pc + 1, s.stack[0 := s.stack[k]][k := s.stack[0]])
-  }
-
-  function SLoad(s: EState): (s': EState)
-    // requires s.IsValid()
-    requires s.Operands() >= 1
-
-    // ensures s'.IsValid()
-    ensures s'.Operands() == s.Operands()
-    // ensures s'.Capacity() == s.Capacity()
-  {
-    EState(s.pc + 1, [Random()] + s.stack[1..])
-  }
-
-  function SStore(s: EState): (s': EState)
-    // requires s.IsValid()
-    requires s.Operands() >= 2
-
-    // ensures s'.IsValid()
-    ensures s'.Operands() == s.Operands() - 2
-    // ensures s'.Capacity() == s.Capacity()
-  {
-    EState(s.pc + 1, s.stack[2..])
-  }
-
-  function MLoad(s: EState): (s': EState)
-    // requires s.IsValid()
-    requires s.Operands() >= 1
-
-    // ensures s'.IsValid()
-    // ensures s'.Operands() == s.Operands()
-    // ensures s'.Capacity() == s.Capacity()
-  {
-    EState(s.pc + 1, [Random()] + s.stack[1..])
-  }
-
-  function MStore(s: EState): (s': EState)
-    // requires s.IsValid()
-    requires s.Operands() >= 2
-
-    // ensures s'.IsValid()
-    // ensures s'.Operands() == s.Operands() - 2
-    // ensures s'.Capacity() == s.Capacity() + 2
-  {
-    EState(s.pc + 1, s.stack[2..])
-  }
-
-  function MStore8(s: EState): (s': EState)
-    // requires s.IsValid()
-    requires s.Operands() >= 2
-
-    // ensures s'.IsValid()
-    // ensures s'.Operands() == s.Operands() - 2
-    // ensures s'.Capacity() == s.Capacity() + 2
-  {
-    EState(s.pc + 1, s.stack[2..])
-  }
-
-  function Jump(s: EState): (s': EState)
-    // requires s.IsValid()
-    requires s.Operands() >= 1
-    requires s.stack[0].Value?
-    // ensures s'.IsValid()
-    // ensures s'.Operands() == s.Operands() - 1
-    // ensures s'.Capacity() == s.Capacity() + 1
-  {
-    EState(s.stack[0].v as nat, s.stack[1..])
-  }
-
-  function JumpI(s: EState): (s': EState)
-    // requires s.IsValid()
-    requires s.Operands() >= 2
-    requires s.stack[0].Value?
-    // ensures s'.IsValid()
-    // ensures s'.Operands() == s.Operands() - 1
-    // ensures s'.Capacity() == s.Capacity() + 1
-    ensures s'.pc == s.stack[0].v as nat || s'.pc == s.pc + 1
-    ensures s'.stack == s.stack[2..]
-//   {
-
-//     EState(if s.stack[1] > 0 then s.stack[0] as nat else s.pc + 1 as nat, s.stack[2..])
-//   }
+  // Arithmetic op
 
   function Add(s: EState): (s': EState)
-    // requires s.IsValid()
     requires s.Operands() >= 2
-    // ensures s'.IsValid()
-    // ensures s'.Operands() == s.Operands() - 1
-    // ensures s'.Capacity() == s.Capacity() + 1
   {
     EState(s.pc + 1, [Random()] + s.stack[2..])
   }
 
   function Sub(s: EState): (s': EState)
-    // requires s.IsValid()
     requires s.Operands() >= 2
-    // ensures s'.IsValid()
-    // ensures s'.Operands() == s.Operands() - 1
-    // ensures s'.Capacity() == s.Capacity() + 1
   {
     EState(s.pc + 1, [Random()] + s.stack[2..])
   }
 
   function Mul(s: EState): (s': EState)
-    // requires s.IsValid()
     requires s.Operands() >= 2
-    // ensures s'.IsValid()
-    // ensures s'.Operands() == s.Operands() - 1
-    // ensures s'.Capacity() == s.Capacity() + 1
   {
     EState(s.pc + 1, [Random()] + s.stack[2..])
   }
 
   function Div(s: EState): (s': EState)
-    // requires s.IsValid()
     requires s.Operands() >= 2
-    // ensures s'.IsValid()
-    // ensures s'.Operands() == s.Operands() - 1
-    // ensures s'.Capacity() == s.Capacity() + 1
+  {
+    EState(s.pc + 1, [Random()] + s.stack[2..])
+  }
+
+  function SDiv(s: EState): (s': EState)
+    requires s.Operands() >= 2
   {
     EState(s.pc + 1, [Random()] + s.stack[2..])
   }
 
   function Mod(s: EState): (s': EState)
-    // requires s.IsValid()
     requires s.Operands() >= 2
-    // ensures s'.IsValid()
-    // ensures s'.Operands() == s.Operands() - 1
-    // ensures s'.Capacity() == s.Capacity() + 1
   {
     EState(s.pc + 1, [Random()] + s.stack[2..])
+  }
+
+  function SMod(s: EState): (s': EState)
+    requires s.Operands() >= 2
+  {
+    EState(s.pc + 1, [Random()] + s.stack[2..])
+  }
+
+  function AddMod(s: EState): (s': EState)
+    requires s.Operands() >= 3
+  {
+    EState(s.pc + 1, [Random()] + s.stack[3..])
+  }
+
+  function MulMod(s: EState): (s': EState)
+    requires s.Operands() >= 3
+  {
+    EState(s.pc + 1, [Random()] + s.stack[3..])
   }
 
   function Exp(s: EState): (s': EState)
-    // requires s.IsValid()
     requires s.Operands() >= 2
-    // ensures s'.IsValid()
-    // ensures s'.Operands() == s.Operands() - 1
-    // ensures s'.Capacity() == s.Capacity() + 1
   {
     EState(s.pc + 1, [Random()] + s.stack[2..])
   }
 
-  function Byte(s: EState): (s': EState)
-    // requires s.IsValid()
+  function SignExtend(s: EState): (s': EState)
     requires s.Operands() >= 2
-    // ensures s'.IsValid()
-    ensures s'.Operands() == s.Operands() - 1
-    // ensures s'.Capacity() == s.Capacity() + 1
   {
     EState(s.pc + 1, [Random()] + s.stack[2..])
   }
+
+  //  Comparison operators
 
   function Lt(s: EState): (s': EState)
-    // requires s.IsValid()
     requires s.Operands() >= 2
-    // ensures s'.IsValid()
-    // ensures s'.Operands() == s.Operands() - 1
-    // ensures s'.Capacity() == s.Capacity() + 1
   {
     EState(s.pc + 1, [Random()] + s.stack[2..])
   }
 
   function Gt(s: EState): (s': EState)
-    // requires s.IsValid()
     requires s.Operands() >= 2
-    // ensures s'.IsValid()
-    // ensures s'.Operands() == s.Operands() - 1
-    // ensures s'.Capacity() == s.Capacity() + 1
   {
     EState(s.pc + 1, [Random()] + s.stack[2..])
   }
 
-  function Slt(s: EState): (s': EState)
-    // requires s.IsValid()
+  function SLt(s: EState): (s': EState)
     requires s.Operands() >= 2
-    // ensures s'.IsValid()
-    // ensures s'.Operands() == s.Operands() - 1
-    // ensures s'.Capacity() == s.Capacity() + 1
   {
     EState(s.pc + 1, [Random()] + s.stack[2..])
   }
 
-   function Sgt(s: EState): (s': EState)
-    // requires s.IsValid()
+  function SGt(s: EState): (s': EState)
     requires s.Operands() >= 2
-    // ensures s'.IsValid()
-    // ensures s'.Operands() == s.Operands() - 1
-    // ensures s'.Capacity() == s.Capacity() + 1
   {
     EState(s.pc + 1, [Random()] + s.stack[2..])
   }
 
   function Eq(s: EState): (s': EState)
-    // requires s.IsValid()
     requires s.Operands() >= 2
-    // ensures s'.IsValid()
-    // ensures s'.Operands() == s.Operands() - 1
-    // ensures s'.Capacity() == s.Capacity() + 1
   {
     EState(s.pc + 1, [Random()] + s.stack[2..])
   }
-
-  function Shr(s: EState): (s': EState)
-    // requires s.IsValid()
-    requires s.Operands() >= 2
-    // ensures s'.IsValid()
-    // ensures s'.Operands() == s.Operands() - 1
-    // ensures s'.Capacity() == s.Capacity() + 1
-  {
-    EState(s.pc + 1, [Random()] + s.stack[2..])
-  }
-
-  function Shl(s: EState): (s': EState)
-    // requires s.IsValid()
-    requires s.Operands() >= 2
-    // ensures s'.IsValid()
-    // ensures s'.Operands() == s.Operands() - 1
-    // ensures s'.Capacity() == s.Capacity() + 1
-  {
-    EState(s.pc + 1, [Random()] + s.stack[2..])
-  }
-
 
   function IsZero(s: EState): (s': EState)
-    // requires s.IsValid()
     requires s.Operands() >= 1
-    // ensures s'.IsValid()
-    // ensures s'.Operands() == s.Operands() - 1
-    // ensures s'.Capacity() == s.Capacity() + 1
   {
     EState(s.pc + 1, [Random()] + s.stack[1..])
   }
 
+  // Bitwise op
+
   function And(s: EState): (s': EState)
-    // requires s.IsValid()
     requires s.Operands() >= 2
-    // ensures s'.IsValid()
-    // ensures s'.Operands() == s.Operands() - 1
-    // ensures s'.Capacity() == s.Capacity() + 1
   {
     EState(s.pc + 1, [Random()] + s.stack[2..])
   }
 
   function Or(s: EState): (s': EState)
-    // requires s.IsValid()
     requires s.Operands() >= 2
-    // ensures s'.IsValid()
-    // ensures s'.Operands() == s.Operands() - 1
-    // ensures s'.Capacity() == s.Capacity() + 1
   {
     EState(s.pc + 1, [Random()] + s.stack[2..])
   }
-
 
   function Xor(s: EState): (s': EState)
-    // requires s.IsValid()
     requires s.Operands() >= 2
-    // ensures s'.IsValid()
-    // ensures s'.Operands() == s.Operands() - 1
-    // ensures s'.Capacity() == s.Capacity() + 1
   {
     EState(s.pc + 1, [Random()] + s.stack[2..])
   }
-
 
   function Not(s: EState): (s': EState)
-    // requires s.IsValid()
     requires s.Operands() >= 1
-    // ensures s'.IsValid()
     ensures s'.Operands() == s.Operands()
-    // ensures s'.Capacity() == s.Capacity() + 1
   {
     EState(s.pc + 1, [Random()] + s.stack[1..])
   }
 
-  function Address(s: EState): (s': EState)
-    // requires s.IsValid()
-    // requires s.Operands() >= 2
-    // requires s.Capacity() >= 1
-    // ensures s'.IsValid()
-    // ensures s'.Operands() == s.Operands() + 1
-    // ensures s'.Capacity() == s.Capacity() - 1
-  {
-    EState(s.pc + 1, [Random()] + s.stack)
-  }
-
-   function Balance(s: EState): (s': EState)
-    // requires s.IsValid()
-    requires s.Operands() >= 1
-    // requires s.Capacity() >= 1
-    // ensures s'.IsValid()
-    ensures s'.Operands() == s.Operands() 
-    // ensures s'.Capacity() == s.Capacity() - 1
-  {
-    EState(s.pc + 1, [Random()] + s.stack[1..])
-  }
-
-   function SelfBalance(s: EState): (s': EState)
-    // requires s.IsValid()
-    // requires s.Operands() >= 1
-    // requires s.Capacity() >= 1
-    // ensures s'.IsValid()
-    ensures s'.Operands() == s.Operands() + 1
-    // ensures s'.Capacity() == s.Capacity() - 1
-  {
-    EState(s.pc + 1, [Random()] + s.stack)
-  }
-
-  function Gas(s: EState): (s': EState)
-    // requires s.IsValid()
-    // requires s.Operands() >= 2
-    // requires s.Capacity() >= 1
-    // ensures s'.IsValid()
-    // ensures s'.Operands() == s.Operands() + 1
-    // ensures s'.Capacity() == s.Capacity() - 1
-  {
-    EState(s.pc + 1, [Random()] + s.stack)
-  }
-
-  function Keccak256(s: EState): (s': EState)
-    // requires s.IsValid()
+  function Byte(s: EState): (s': EState)
     requires s.Operands() >= 2
-    // requires s.Capacity() >= 1
-    // ensures s'.IsValid()
     ensures s'.Operands() == s.Operands() - 1
-    // ensures s'.Capacity() == s.Capacity() - 1
   {
     EState(s.pc + 1, [Random()] + s.stack[2..])
+  }
+
+  function Shr(s: EState): (s': EState)
+    requires s.Operands() >= 2
+  {
+    EState(s.pc + 1, [Random()] + s.stack[2..])
+  }
+
+  function Shl(s: EState): (s': EState)
+    requires s.Operands() >= 2
+  {
+    EState(s.pc + 1, [Random()] + s.stack[2..])
+  }
+
+  function Sar(s: EState): (s': EState)
+    requires s.Operands() >= 2
+  {
+    EState(s.pc + 1, [Random()] + s.stack[2..])
+  }
+
+  //  Keccak256
+
+  function Keccak256(s: EState): (s': EState)
+    requires s.Operands() >= 2
+  {
+    EState(s.pc + 1, [Random()] + s.stack[2..])
+  }
+
+  //  Env op
+
+  function Address(s: EState): (s': EState)
+  {
+    EState(s.pc + 1, [Random()] + s.stack)
+  }
+
+  function Balance(s: EState): (s': EState)
+    requires s.Operands() >= 1
+  {
+    EState(s.pc + 1, [Random()] + s.stack[1..])
+  }
+
+  function Origin(s: EState): (s': EState)
+  {
+    EState(s.pc + 1, [Random()] + s.stack)
+  }
+
+  function Caller(s: EState): (s': EState)
+  {
+    EState(s.pc + 1, [Random()] + s.stack)
   }
 
   function CallValue(s: EState): (s': EState)
-    // requires s.IsValid()
-    // requires s.Capacity() >= 1
-    // ensures s'.IsValid()
-    // ensures s'.Operands() == s.Operands()
-    // ensures s'.Capacity() == s.Capacity()
   {
     EState(s.pc + 1, [Random()] + s.stack)
   }
 
   function CallDataLoad(s: EState): (s': EState)
-    // requires s.IsValid()
     requires s.Operands() >= 1
-    // ensures s'.IsValid()
-    // ensures s'.Operands() == s.Operands()
-    // ensures s'.Capacity() == s.Capacity()
   {
     EState(s.pc + 1, [Random()] + s.stack[1..])
   }
 
+  function CallDataSize(s: EState): (s': EState)
+  {
+    EState(s.pc + 1, [Random()] + s.stack)
+  }
+
   function CallDataCopy(s: EState): (s': EState)
-    // requires s.IsValid()
     requires s.Operands() >= 3
-    // ensures s'.IsValid()
-    // ensures s'.Operands() == s.Operands() - 3
-    // ensures s'.Capacity() == s.Capacity() + 3
   {
     EState(s.pc + 1, s.stack[3..])
+  }
+
+  function CodeSize(s: EState): (s': EState)
+  {
+    EState(s.pc + 1, [Random()] + s.stack)
   }
 
   function CodeCopy(s: EState): (s': EState)
-    // requires s.IsValid()
     requires s.Operands() >= 3
-    // ensures s'.IsValid()
-    ensures s'.Operands() == s.Operands() - 3
-    // ensures s'.Capacity() == s.Capacity() + 3
   {
     EState(s.pc + 1, s.stack[3..])
   }
 
-  function CallDataSize(s: EState): (s': EState)
-    // requires s.IsValid()
-    // requires s.Capacity() >= 1
-    // ensures s'.IsValid()
-    // ensures s'.Operands() == s.Operands() - 3
-    // ensures s'.Capacity() == s.Capacity() + 3
+  function GasPrice(s: EState): (s': EState)
   {
     EState(s.pc + 1, [Random()] + s.stack)
   }
 
   function ExtCodeSize(s: EState): (s': EState)
-    // requires s.IsValid()
     requires s.Operands() >= 1
-    // ensures s'.IsValid()
-    ensures s'.Operands() == s.Operands()
-    // ensures s'.Capacity() == s.Capacity() + 3
   {
     EState(s.pc + 1, [Random()] + s.stack[1..])
   }
-  function Caller(s: EState): (s': EState)
-    // requires s.IsValid()
-    // requires s.Capacity() >= 1
-    // ensures s'.IsValid()
-    // ensures s'.Operands() == s.Operands() + 1
-    // ensures s'.Capacity() == s.Capacity() - 1
-    ensures s'.stack == [Random()] + s.stack
+
+  function ExtCodeCopy(s: EState): (s': EState)
+    requires s.Operands() >= 4
   {
-    EState(s.pc + 1, [Random()] + s.stack)
+    EState(s.pc + 1, s.stack[4..])
   }
 
   function ReturnDataSize(s: EState): (s': EState)
-    // requires s.IsValid()
-    // requires s.Capacity() >= 1
-    // ensures s'.IsValid()
-    ensures s'.Operands() == s.Operands() + 1
-    // ensures s'.Capacity() == s.Capacity() + 3
   {
     EState(s.pc + 1, [Random()] + s.stack)
   }
 
   function ReturnDataCopy(s: EState): (s': EState)
-    // requires s.IsValid()
     requires s.Operands() >= 3
-    // ensures s'.IsValid()
-    ensures s'.Operands() == s.Operands() - 3
-    // ensures s'.Capacity() == s.Capacity() + 3
   {
     EState(s.pc + 1, s.stack[3..])
   }
 
+  function ExtCodeHash(s: EState): (s': EState)
+    requires s.Operands() >= 1
+  {
+    EState(s.pc + 1, [Random()] + s.stack[1..])
+  }
+
+  //  Block information
+
+  function BlockHash(s: EState): (s': EState)
+    requires s.Operands() >= 1
+  {
+    EState(s.pc + 1, [Random()] + s.stack[1..])
+  }
+
+  function CoinBase(s: EState): (s': EState)
+  {
+    EState(s.pc + 1, [Random()] + s.stack)
+  }
+
+  function TimeStamp(s: EState): (s': EState)
+  {
+    EState(s.pc + 1, [Random()] + s.stack)
+  }
+
+  function Number(s: EState): (s': EState)
+  {
+    EState(s.pc + 1, [Random()] + s.stack)
+  }
+
+  function Difficulty(s: EState): (s': EState)
+  {
+    EState(s.pc + 1, [Random()] + s.stack)
+  }
+
+  function GasLimit(s: EState): (s': EState)
+  {
+    EState(s.pc + 1, [Random()] + s.stack)
+  }
+
+  function ChainID(s: EState): (s': EState)
+  {
+    EState(s.pc + 1, [Random()] + s.stack)
+  }
+
+  function SelfBalance(s: EState): (s': EState)
+    ensures s'.Operands() == s.Operands() + 1
+  {
+    EState(s.pc + 1, [Random()] + s.stack)
+  }
+
+  function BaseFee(s: EState): (s': EState)
+    ensures s'.Operands() == s.Operands() + 1
+  {
+    EState(s.pc + 1, [Random()] + s.stack)
+  }
+
+  // 0x50s: Stack, Memory, Storage and Flow
+
+  function Pop(s: EState): (s': EState)
+    requires s.Operands() >= 1
+  {
+    EState(s.pc + 1, s.stack[1..])
+  }
+
+  function MLoad(s: EState): (s': EState)
+    requires s.Operands() >= 1
+  {
+    EState(s.pc + 1, [Random()] + s.stack[1..])
+  }
+
+  function MStore(s: EState): (s': EState)
+    requires s.Operands() >= 2
+  {
+    EState(s.pc + 1, s.stack[2..])
+  }
+
+  function MStore8(s: EState): (s': EState)
+    requires s.Operands() >= 2
+  {
+    EState(s.pc + 1, s.stack[2..])
+  }
+
+  function SLoad(s: EState): (s': EState)
+    requires s.Operands() >= 1
+  {
+    EState(s.pc + 1, [Random()] + s.stack[1..])
+  }
+
+  function SStore(s: EState): (s': EState)
+    requires s.Operands() >= 2
+    ensures s'.Operands() == s.Operands() - 2
+  {
+    EState(s.pc + 1, s.stack[2..])
+  }
+
+  function Jump(s: EState): (s': EState)
+    requires s.Operands() >= 1
+    requires s.stack[0].Value?
+  {
+    EState(s.stack[0].v as nat, s.stack[1..])
+  }
+
+  // The semantics of JumpI is non-deterninisitic and can lead to
+  //    to two different state.
+  function JumpI(s: EState): (s': EState)
+    requires s.Operands() >= 2
+    requires s.stack[0].Value?
+    ensures s'.pc == s.stack[0].v as nat || s'.pc == s.pc + 1
+    ensures s'.stack == s.stack[2..]
+
+  // RJUMPs, PC not supported,
+
+  function MSize(s: EState): (s': EState)
+  {
+    EState(s.pc + 1, [Random()] + s.stack)
+  }
+
+  function Gas(s: EState): (s': EState)
+  {
+    EState(s.pc + 1, [Random()] + s.stack)
+  }
+
   function JumpDest(s: EState): (s': EState)
-    // requires s.IsValid()
-    // requires s.Capacity() >= 1
-    // ensures s'.IsValid()
-    // ensures s'.Operands() == s.Operands() + 1
-    // ensures s'.Capacity() == s.Capacity() - 1
-    // ensures s'.stack == [Random()] + s.stack
   {
     EState(s.pc + 1, s.stack)
   }
 
-  function Revert(s: EState): (s': EState)
-    // requires s.IsValid()
-    // requires s.Capacity() >= 1
-    // ensures s'.IsValid()
-    // ensures s'.Operands() == s.Operands() + 1
-    // ensures s'.Capacity() == s.Capacity() - 1
-    // ensures s'.stack == [Random()] + s.stack
+  function Push0(s: EState): (s': EState)
+    ensures s'.Operands() == s.Operands() + 1
+    ensures s'.stack[1..] == s.stack
   {
-    EState(s.pc + 1, s.stack)
+    EState(s.pc + 1, [Random()] + s.stack)
   }
 
-  function Return(s: EState): (s': EState)
-    // requires s.IsValid()
-    // requires s.Capacity() >= 1
-    // ensures s'.IsValid()
-    // ensures s'.Operands() == s.Operands() + 1
-    // ensures s'.Capacity() == s.Capacity() - 1
-    // ensures s'.stack == [Random()] + s.stack
+  // 0x60s & 0x70s: Push operations
+  function PushN(s: EState, n: nat, k: nat): (s': EState)
+    requires 1 <= n <= 32
+    requires k <= Int.MAX_U256
+    ensures s'.Operands() == s.Operands() + 1
+    ensures s'.stack[1..] == s.stack
   {
-    EState(s.pc + 1, s.stack)
+    EState(s.pc + n + 1, [Value(k as Int.u256)] + s.stack)
   }
 
-  function Stop(s: EState): (s': EState)
-    // requires s.IsValid()
-    // requires s.Capacity() >= 1
-    // ensures s'.IsValid()
-    // ensures s'.Operands() == s.Operands() + 1
-    // ensures s'.Capacity() == s.Capacity() - 1
-    // ensures s'.stack == [Random()] + s.stack
+  function Dup(s: EState, k: nat): (s': EState)
+    requires s.Operands() >= k > 0
+    ensures s'.stack == [s.stack[k - 1]] + s.stack
   {
-    EState(s.pc + 1, s.stack)
+    EState(s.pc + 1, [s.stack[k - 1]] + s.stack)
   }
 
+  function Swap(s: EState, k: nat): (s': EState)
+    requires 1 <= k <= 16
+    requires s.Operands() > k
+  {
+    EState(s.pc + 1, s.stack[0 := s.stack[k]][k := s.stack[0]])
+  }
 
+  //  Log op
   function LogN(s: EState, n: nat): (s': EState)
     requires n <= 4
-    // requires s.IsValid()
     requires s.Operands() >= n + 2
-    // ensures s'.IsValid()
     ensures s'.Operands() == s.Operands() - (n + 2)
-    // ensures s'.Capacity() == s.Capacity() - 1
-    // ensures s'.stack == [Random()] + s.stack
   {
     EState(s.pc + 1, s.stack[n + 2..])
   }
 
+  //  System op
+
+  function Create(s: EState): (s': EState)
+    requires s.Operands() >= 3
+  {
+    EState(s.pc + 1, [Random()] + s.stack[3..])
+  }
+
+  function Call(s: EState): (s': EState)
+    requires s.Operands() >= 7
+  {
+    EState(s.pc + 1, [Random()] + s.stack[7..])
+  }
+
+  function CallCode(s: EState): (s': EState)
+    requires s.Operands() >= 7
+  {
+    EState(s.pc + 1, [Random()] + s.stack[7..])
+  }
+
+  function Return(s: EState): (s': EState)
+  {
+    EState(s.pc + 1, s.stack)
+  }
+
+  function DelegateCall(s: EState): (s': EState)
+    requires s.Operands() >= 6
+  {
+    EState(s.pc + 1, [Random()] + s.stack[6..])
+  }
+
+  function Create2(s: EState): (s': EState)
+    requires s.Operands() >= 4
+  {
+    EState(s.pc + 1, [Random()] + s.stack[4..])
+  }
+
+  function StaticCall(s: EState): (s': EState)
+    requires s.Operands() >= 6
+  {
+    EState(s.pc + 1, [Random()] + s.stack[6..])
+  }
+
+  function Revert(s: EState): (s': EState)
+  {
+    EState(s.pc + 1, s.stack)
+  }
+
+  function SelfDestruct(s: EState): (s': EState)
+    requires s.Operands() >= 1
+  {
+    EState(s.pc + 1, s.stack[1..])
+  }
 
 }
